Move security proof of copy-mac-cache

casestudy/copy_mac_cache_ct_proof.ec
@@ -1,17 +1,33 @@
 require import AllCore IntDiv CoreMap List.
 from Jasmin require import JModel.
 
-require import Array128 WArray128 Lucky13_split_full_log_proof Lucky13_split_div64_log.
+require import Array128 WArray128.
+
+require Copy_mac_ct.
+
+theory LeakageModelCL.
+
+op leak_div_32 (a b: W32.t) : address list = [].
+
+op leak_div_64 (a b: W64.t) : address list = [].
+
+op leak_mem (a: address) : address =
+  a %/ 64.
+
+end LeakageModelCL.
+
+clone import Copy_mac_ct.T with
+theory LeakageModel <- LeakageModelCL.
 
 equiv l_rotate_offset_div md_size_ : M.rotate_offset_div ~ M.rotate_offset_div:
 ={M.leakages, md_size, scan_start} /\ md_size{1} = md_size_ /\
-(0 <= (to_uint (mac_start - scan_start)) < 2^8){1} /\ 
+(0 <= (to_uint (mac_start - scan_start)) < 2^8){1} /\
 (0 <= (to_uint (mac_start - scan_start)) < 2^8){2} /\
 (16 <= to_uint md_size <= 64){1}
 ==> ={M.leakages} /\ 0 <= to_uint res{1} < to_uint md_size_ /\ 0 <= to_uint res{2} < to_uint md_size_.
 proof.
   proc; wp; skip => /> *.
-  rewrite !l_rotate_offset_div_core //= W32.umodE /ulift2 /=; smt (W32.to_uint_small W32.to_uint_cmp).
+  smt (W32.to_uint_small W32.to_uint_cmp).
 qed.
 
 (* md_size : mac tag size --> public *)
@@ -19,65 +35,65 @@ qed.
 (* out : mac tag is stored in out --> public *)
 (* rec : whole message including header, message, tag, padding --> public *)
 
-op wf_rec mem (rec:W64.t) (orig_len md_size : W32.t) = 
+op wf_rec mem (rec:W64.t) (orig_len md_size : W32.t) =
  let mac_end = loadW32 mem (to_uint (rec + W64.of_int 4)) in
- to_uint md_size <= to_uint mac_end /\ 
+ to_uint md_size <= to_uint mac_end /\
  1 <= to_uint orig_len - to_uint mac_end <= 256.
 
-lemma wf_rec_cond_md_size_mac_end mem rec orig_len md_size : 
+lemma wf_rec_cond_md_size_mac_end mem rec orig_len md_size :
   16 <= W32.to_uint md_size <= 64 =>
   wf_rec mem rec orig_len md_size =>
   let mac_end = loadW32 mem (to_uint (rec + W64.of_int 4)) in
-  if (md_size + W32.of_int 256 \ult orig_len) then 
+  if (md_size + W32.of_int 256 \ult orig_len) then
      0 <= to_uint (mac_end - md_size - (orig_len - (md_size + W32.of_int 256))) < 256
   else 0 <= to_uint (mac_end - md_size - W32.zero) < 256.
 proof.
   rewrite /wf_rec /=.
   pose mac_end := loadW32 _ _; move: mac_end => mac_end hmd [h1 [h2 h3]].
-  have -> : mac_end - md_size - (orig_len - (md_size + W32.of_int 256)) = 
+  have -> : mac_end - md_size - (orig_len - (md_size + W32.of_int 256)) =
             mac_end - (orig_len - W32.of_int 256) by ring.
   rewrite W32.ultE W32.to_uintD_small /= 1:/#.
   case: (to_uint md_size + 256 < to_uint orig_len) => h; last first.
   + rewrite W32.WRingA.subr0 W32.to_uintB 1:W32.uleE 1:// /#.
-  rewrite W32.to_uintB ?W32.uleE W32.to_uintB ?W32.uleE /=; smt(W32.to_uint_cmp). 
+  rewrite W32.to_uintB ?W32.uleE W32.to_uintB ?W32.uleE /=; smt(W32.to_uint_cmp).
 qed.
 
-lemma offset_div (p:W64.t) (offset: W32.t): 
-  to_uint p + 64 <= W64.modulus => 
-  64 %| to_uint p => 
-  0 <= to_uint offset < 64 => 
+lemma offset_div (p:W64.t) (offset: W32.t):
+  to_uint p + 64 <= W64.modulus =>
+  64 %| to_uint p =>
+  0 <= to_uint offset < 64 =>
   to_uint (p + zeroextu64 offset) %/ 64  = to_uint p %/ 64.
 proof.
   move=> /= h1 h2 h3; rewrite W64.to_uintD_small to_uint_zeroextu64 /= 1:/# divzDl 1:// /#.
 qed.
 
-equiv l_rotate_mac_ct : M.rotate_mac_cache ~ M.rotate_mac_cache : 
+equiv l_rotate_mac_ct : M.rotate_mac_cache ~ M.rotate_mac_cache :
   ={M.leakages, out, md_size, rotated_mac} /\ 64 %| W64.to_uint rotated_mac{1} /\
   to_uint rotated_mac{1} + 64 <= W64.modulus /\
   16 <= to_uint md_size{1} <= 64 /\
   0 <= to_uint rotate_offset{1} < to_uint md_size{1}  /\ 0 <= to_uint rotate_offset{2} < to_uint md_size{1}
-  ==> 
+  ==>
   ={M.leakages}.
 proof.
   proc.
-  while (={out, rotated_mac, md_size, i, j, M.leakages} /\ 64 %| W64.to_uint rotated_mac{1} /\
+  while (={out, rotated_mac, md_size, i, M.leakages} /\ 64 %| W64.to_uint rotated_mac{1} /\
          to_uint rotated_mac{1} + 64 <= W64.modulus /\
-         16 <= to_uint md_size{1} <= 64 /\ 
+         16 <= to_uint md_size{1} <= 64 /\
          0 <= to_uint rotate_offset{1} < to_uint md_size{1}  /\ 0 <= to_uint rotate_offset{2} < to_uint md_size{1}).
   + inline *; wp; skip => /> &1 &2 hmod nover h1 h2 h3 h4 h5 h6 hi.
-    rewrite !offset_div //= 1,2:/#.
+    rewrite /leak_mem !offset_div //= 1,2:/#.
     split; rewrite uleE.
     + case: (to_uint md_size{2} <= to_uint (rotate_offset{1} + W32.one)) => /=; smt(W32.to_uint_cmp).
     case: (to_uint md_size{2} <= to_uint (rotate_offset{2} + W32.one)) => /=; smt(W32.to_uint_cmp).
-  by wp; skip => />. 
+  by wp; skip => />.
 qed.
-print (%|).
+
 equiv l_final : M.ssl3_cbc_copy_mac_jasmin_cache ~ M.ssl3_cbc_copy_mac_jasmin_cache :
 ={M.leakages, md_size, orig_len, out, rec, rotated_mac} /\
 (loadW64 Glob.mem (to_uint (rec + (of_int 16)%W64))){1} = (loadW64 Glob.mem (to_uint (rec + (of_int 16)%W64))){2} /\
 to_uint rotated_mac{2} + 64 <= W64.modulus /\ 64 %| to_uint rotated_mac{2} /\
 16 <= to_uint md_size{2} <= 64 /\
-(wf_rec Glob.mem rec orig_len md_size){1} /\ (wf_rec Glob.mem rec orig_len md_size){2}  
+(wf_rec Glob.mem rec orig_len md_size){1} /\ (wf_rec Glob.mem rec orig_len md_size){2}
 ==> ={M.leakages}.
 proof.
   proc.
@@ -87,4 +103,3 @@ proof.
   wp => /=; while (={i, rotated_mac, md_size, M.leakages}); 1: by sim.
   wp; skip => |> &1 &2; smt (wf_rec_cond_md_size_mac_end).
 qed.
-
